src/typechecker/FStar.TypeChecker.NBETerm.fst
@@ -660,7 +660,7 @@ let binary_bool_op (f:bool -> bool -> bool) =
 let binary_string_op (f : string -> string -> string) =
     binary_op arg_as_string (fun x y -> embed e_string bogus_cbs (f x y))
 
-let mixed_binary_op (as_a : arg -> option 'a) (as_b : arg -> option 'b)
+let mixed_binary_op_no_univs (as_a : arg -> option 'a) (as_b : arg -> option 'b)
        (embed_c : 'c -> t) (f : 'a -> 'b -> option 'c) (args : args) : option t =
              match args with
              | [a;b] ->
@@ -674,18 +674,34 @@ let mixed_binary_op (as_a : arg -> option 'a) (as_b : arg -> option 'b)
                 end
              | _ -> None
 
+let mixed_binary_op (as_a : arg -> option 'a) (as_b : arg -> option 'b)
+       (embed_c : 'c -> t) (f : universes -> 'a -> 'b -> option 'c)
+       (us:universes) (args : args) : option t =
+             match args with
+             | [a;b] ->
+                begin
+                match as_a a, as_b b with
+                | Some a, Some b ->
+                  (match f us a b with
+                   | Some c -> Some (embed_c c)
+                   | _ -> None)
+                | _ -> None
+                end
+             | _ -> None
+
 let mixed_ternary_op (as_a : arg -> option 'a)
                      (as_b : arg -> option 'b)
                      (as_c : arg -> option 'c)                     
                      (embed_d : 'd -> t) 
-                     (f : 'a -> 'b -> 'c -> option 'd)
+                     (f : universes -> 'a -> 'b -> 'c -> option 'd)
+                     (us: universes)
                      (args : args) : option t =
              match args with
              | [a;b;c] ->
                 begin
                 match as_a a, as_b b, as_c c with
                 | Some a, Some b, Some c ->
-                  (match f a b c with
+                  (match f us a b c with
                    | Some d -> Some (embed_d d)
                    | _ -> None)
                 | _ -> None
