src/tactics/FStar.Tactics.Interpreter.fst
@@ -66,8 +66,8 @@ let native_tactics_steps () =
     ; Cfg.auto_reflect                 = Some (s.arity - 1)
     ; Cfg.strong_reduction_ok          = s.strong_reduction_ok
     ; Cfg.requires_binder_substitution = false // GM: Don't think we care about pretty-printing on native
-    ; Cfg.interpretation               = s.tactic
-    ; Cfg.interpretation_nbe           = fun _cb -> NBET.dummy_interp s.name
+    ; Cfg.interpretation               = (fun psc cb _us t -> s.tactic psc cb t)
+    ; Cfg.interpretation_nbe           = fun _cb _us -> NBET.dummy_interp s.name
     }
   in
   List.map step_from_native_step (Native.list_all ())
