src/typechecker/FStar.TypeChecker.NBETerm.fsti
@@ -339,14 +339,19 @@ val list_of_string' : (string -> t)
 val decidable_eq : bool -> args -> option t
 val interp_prop_eq2 : args -> option t
 
+val mixed_binary_op_no_univs :
+    (arg -> option 'a) -> (arg -> option 'b) -> ('c -> t) ->
+    ('a -> 'b -> option 'c) -> args -> option t
+
 val mixed_binary_op : (arg -> option 'a) -> (arg -> option 'b) -> ('c -> t) ->
-                      ('a -> 'b -> option 'c) -> args -> option t
+                      (universes -> 'a -> 'b -> option 'c) -> universes -> args -> option t
 
 val mixed_ternary_op (as_a : arg -> option 'a)
                      (as_b : arg -> option 'b)
                      (as_c : arg -> option 'c)                     
                      (embed_d : 'd -> t) 
-                     (f : 'a -> 'b -> 'c -> option 'd)
+                     (f : universes -> 'a -> 'b -> 'c -> option 'd)
+                     (us:universes)
                      (args : args) : option t
 
 val unary_op : (arg -> option 'a) -> ('a -> t) -> (args -> option t)
